refactor: remove the Solver structure

LeanSAT/Reflect/Tactics/CNFDecide.lean
@@ -1,7 +1,7 @@
 /-
 Copyright (c) 2024 Lean FRO, LLC. All rights reserved.
 Released under Apache 2.0 license as described in the file LICENSE.
-Authors: Scott Morrison
+Authors: Scott Morrison, Henrik Böving
 -/
 import LeanSAT.Reflect.Tactics.Reflect
 import LeanSAT.Reflect.BoolExpr.Tseitin.Lemmas
@@ -13,62 +13,27 @@ import LeanSAT.External.Solver
 
 open Lean Elab Meta ReflectSat
 
-structure TacticConfig where
+namespace CnfDecide
+
+/--
+The context for the `cnf_decide` tactic.
+-/
+structure TacticContext where
   boolExprDef : Name
   certDef : Name
   reflectionDef : Name
 
 /--
-Interface for an external SAT solver with a verified certificate checker.
-
-The type `α` representing the specific encoding of `CNF Nat` that the `Solver`
-backend uses.
-
-The type `β` representing the unsatisfiability certificate should have `ToExpr β`,
-because we will need to embed the certificate in the generated proof.
--/
-structure Solver (α : Type) (β : Type) where
-  /-- Encode the generic `CNF Nat` into the `Solver` specific CNF format. -/
-  encodeCNF : CNF Nat → α
-  /-- An IO function that retrieves an opaque certificate of type `β`. -/
-  runExternal : α → IO β
-  /--
-  A verification function,
-  where `verify (encodeCNF c) b = true` if `b` is a valid certificate of the unsatisfiability of `c`.
-  -/
-  verify : α → β → Bool
-  /-- Proof of the correctness of the verification function. -/
-  correct : ∀ c b, verify (encodeCNF c) b = true → c.unsat
-
-def Solver.verifyExpr (s : Solver α β) (b : BoolExpr Nat) (c : β) : Bool :=
-  s.verify (s.encodeCNF b.toCNF) c
-
-theorem Solver.unsat_of_verifyExpr_eq_true (s : Solver α β) (b : BoolExpr Nat) (c : β)
-    (h : s.verifyExpr b c = true) : BoolExpr.unsat b := by
-  apply BoolExpr.unsat_of_toCNF_unsat
-  apply s.correct
-  rw [verifyExpr] at h
-  exact h
-
-/--
-A wrapper type for `LRAT.DefaultFormula`. We use it to hide the `numVars` parameter
-as the `Solver` framework does not intend for dependent typing like this.
+A wrapper type for `LRAT.DefaultFormula`. We use it to hide the `numVars` parameter.
 -/
 structure LratFormula where
   /-- Number of variables in `formula`. -/
-  numVars : Nat
+  {numVars : Nat}
   /-- The actual SAT formula in the LeanSAT framework. -/
   formula : LRAT.DefaultFormula numVars.succ
 
-/--
-An LRAT proof certificate. Note that this only contains a list of LRAT actions
-that have not yet been internalized to the formats that LeanSAT's LRAT checker uses.
-This is done as we need to provide an `ToExpr LratCert` instance, which not easily
-possible for proof carrying structures.
--/
-structure LratCert where
-  /-- An LRAT proof read from a file. This will get parsed using ofReduceBool. -/
-  cert : String
+/-- An LRAT proof read from a file. This will get parsed using ofReduceBool. -/
+abbrev LratCert := String
 
 instance : ToExpr LRAT.IntAction where
   toExpr action :=
@@ -85,108 +50,136 @@ instance : ToExpr LRAT.IntAction where
       mkApp3 (mkConst ``LRAT.Action.del [.zero, .zero]) beta alpha (toExpr ids)
   toTypeExpr := mkConst ``LRAT.IntAction
 
-instance : ToExpr LratCert where
-  toExpr cert := mkApp (mkConst ``LratCert.mk) (toExpr cert.cert)
-  toTypeExpr := mkConst ``LratCert
 
+/--
+Turn a `CNF` from the reflection framework into the correct format for the LRAT framework.
+-/
+def LratFormula.ofCnf (cnf : CNF Nat) : LratFormula := ⟨cnf.convertLRAT⟩
+
+/--
+Create a temporary file using `mktemp` and return the path to it.
+-/
 def mkTemp : IO System.FilePath := do
   let out ← IO.Process.output { cmd := "mktemp" }
   return out.stdout.trim
 
-def lratSolver : Solver LratFormula LratCert where
-  encodeCNF reflectCnf :=
-    ⟨_, reflectCnf.convertLRAT⟩
+/--
+Run an external SAT solver on the `LratFormula` to obtain an LRAT proof.
 
-  runExternal formula := do
-    let formula := formula.formula
-    -- TODO: In the future we might want to cache these
-    let cnfPath ← mkTemp
-    let lratPath ← mkTemp
-    IO.FS.writeFile cnfPath <| formula.dimacs
-    -- TODO: make cadical parameterizable
-    satQuery "cadical" cnfPath lratPath
-    let lines ← IO.FS.lines lratPath
-    -- This is just a sanity check to verify that the proof does indeed parse.
-    -- The parsing relevant for the reflection proof happens in the reflection term.
-    if LRAT.parseLRATProof lines |>.isNone then
-      throw <| IO.userError "SAT solver produced invalid LRAT"
-    -- cleanup files such that we don't pollute /tmp
-    IO.FS.removeFile cnfPath
-    IO.FS.removeFile lratPath
-    -- XXX String.intercalate wit Array
-    let lratProof := String.intercalate "\n" lines.toList
-    return ⟨lratProof⟩
+This will obtain an `LratCert` if the formula is UNSAT and throw errors otherwise.
+-/
+def runExternal (formula : LratFormula) : IO LratCert := do
+  let formula := formula.formula
+  -- TODO: In the future we might want to cache these
+  let cnfPath ← mkTemp
+  let lratPath ← mkTemp
+  IO.FS.writeFile cnfPath <| formula.dimacs
+  -- TODO: make cadical parameterizable
+  satQuery "cadical" cnfPath lratPath
+  let lines ← IO.FS.lines lratPath
+  -- This is just a sanity check to verify that the proof does indeed parse.
+  -- The parsing relevant for the reflection proof happens in the reflection term.
+  if LRAT.parseLRATProof lines |>.isNone then
+    throw <| IO.userError "SAT solver produced invalid LRAT"
+  -- cleanup files such that we don't pollute /tmp
+  IO.FS.removeFile cnfPath
+  IO.FS.removeFile lratPath
+  -- XXX String.intercalate wit Array
+  let lratProof := String.intercalate "\n" lines.toList
+  return lratProof
 
-  verify formula cert :=
-    -- XXX String.splitOn with Array
-    let lines := cert.cert.splitOn "\n" |>.toArray
-    match LRAT.parseLRATProof lines with
-    | some lratProof =>
-      -- XXX
-      let lratProof := lratProof.toList
-      let lratProof := lratProof.map (LRAT.intActionToDefaultClauseAction formula.numVars.succ)
-      let lratProof : List { act // LRAT.wellFormedAction act } :=
-        lratProof.filterMap
-          (fun actOpt =>
-            match actOpt with
-            | none => none
-            | some (LRAT.Action.addEmpty id rupHints) =>
-              some ⟨LRAT.Action.addEmpty id rupHints, by simp only [LRAT.wellFormedAction]⟩
-            | some (LRAT.Action.addRup id c rupHints) =>
-              some ⟨LRAT.Action.addRup id c rupHints, by simp only [LRAT.wellFormedAction]⟩
-            | some (LRAT.Action.del ids) =>
-              some ⟨LRAT.Action.del ids, by simp only [LRAT.wellFormedAction]⟩
-            | some (LRAT.Action.addRat id c pivot rupHints ratHints) =>
-              if h : pivot ∈ LRAT.Clause.toList c then
-                some ⟨
-                  LRAT.Action.addRat id c pivot rupHints ratHints,
-                  by simp [LRAT.wellFormedAction, LRAT.Clause.limplies_iff_mem, h]
-                ⟩
-              else
-                -- TODO: report this
-                none
-          )
-      let lratProof := lratProof.map Subtype.val
-      let checkerResult := LRAT.lratChecker formula.formula lratProof
-      checkerResult = .success
-    | none => false
+/--
+Verify that a proof certificate is valid for a given formula.
+-/
+def verifyCert (formula : LratFormula) (cert : LratCert) : Bool :=
+  -- XXX String.splitOn with Array
+  let lines := cert.splitOn "\n" |>.toArray
+  match LRAT.parseLRATProof lines with
+  | some lratProof =>
+    -- XXX
+    let lratProof := lratProof.toList
+    let lratProof := lratProof.map (LRAT.intActionToDefaultClauseAction formula.numVars.succ)
+    let lratProof : List { act // LRAT.wellFormedAction act } :=
+      lratProof.filterMap
+        (fun actOpt =>
+          match actOpt with
+          | none => none
+          | some (LRAT.Action.addEmpty id rupHints) =>
+            some ⟨LRAT.Action.addEmpty id rupHints, by simp only [LRAT.wellFormedAction]⟩
+          | some (LRAT.Action.addRup id c rupHints) =>
+            some ⟨LRAT.Action.addRup id c rupHints, by simp only [LRAT.wellFormedAction]⟩
+          | some (LRAT.Action.del ids) =>
+            some ⟨LRAT.Action.del ids, by simp only [LRAT.wellFormedAction]⟩
+          | some (LRAT.Action.addRat id c pivot rupHints ratHints) =>
+            if h : pivot ∈ LRAT.Clause.toList c then
+              some ⟨
+                LRAT.Action.addRat id c pivot rupHints ratHints,
+                by simp [LRAT.wellFormedAction, LRAT.Clause.limplies_iff_mem, h]
+              ⟩
+            else
+              -- TODO: report this
+              none
+        )
+    let lratProof := lratProof.map Subtype.val
+    let checkerResult := LRAT.lratChecker formula.formula lratProof
+    checkerResult = .success
+  | none => false
 
-  correct := by
-    intro c b h1
-    dsimp at h1
-    split at h1
-    . simp only [decide_eq_true_eq] at h1
-      have h2 :=
-        lratCheckerSound
-          _
-          (by apply CNF.convertLRAT_readfyForRupAdd)
-          (by apply CNF.convertLRAT_readfyForRatAdd)
-          _
-          (by
-            intro action h
-            simp only [List.mem_map, List.mem_filterMap] at h
-            rcases h with ⟨wellFormedActions, _, h2⟩
-            rw [← h2]
-            exact wellFormedActions.property)
-          h1
-      apply CNF.unsat_of_lift_unsat c
-      intro assignment
-      unfold CNF.convertLRAT at h2
-      have h2 := (LRAT.unsat_of_cons_none_unsat _ h2) assignment
-      apply eq_false_of_ne_true
-      intro h3
-      apply h2
-      simp only [LRAT.Formula.formulaHSat_def, List.all_eq_true, decide_eq_true_eq]
-      intro lratClause hlclause
-      simp only [LRAT.Formula.toList, LRAT.DefaultFormula.toList, LRAT.DefaultFormula.ofArray,
-        CNF.convertLRAT', Array.size_toArray, List.length_map, Array.toList_eq, Array.data_toArray,
-        List.map_nil, List.append_nil, List.mem_filterMap, List.mem_map, id_eq, exists_eq_right] at hlclause
-      rcases hlclause with ⟨reflectClause, ⟨hrclause1, hrclause2⟩⟩
-      simp only [CNF.eval, List.all_eq_true] at h3
-      simp [CNF.Clause.convertLRAT_sat_of_sat reflectClause hrclause2, h3 reflectClause hrclause1]
-    . contradiction
+theorem verifyCert_correct : ∀ cnf cert, verifyCert (LratFormula.ofCnf cnf) cert = true → cnf.unsat := by
+  intro c b h1
+  dsimp[verifyCert] at h1
+  split at h1
+  . simp only [decide_eq_true_eq] at h1
+    have h2 :=
+      lratCheckerSound
+        _
+        (by apply CNF.convertLRAT_readfyForRupAdd)
+        (by apply CNF.convertLRAT_readfyForRatAdd)
+        _
+        (by
+          intro action h
+          simp only [List.mem_map, List.mem_filterMap] at h
+          rcases h with ⟨wellFormedActions, _, h2⟩
+          rw [← h2]
+          exact wellFormedActions.property)
+        h1
+    apply CNF.unsat_of_lift_unsat c
+    intro assignment
+    unfold CNF.convertLRAT at h2
+    have h2 := (LRAT.unsat_of_cons_none_unsat _ h2) assignment
+    apply eq_false_of_ne_true
+    intro h3
+    apply h2
+    simp only [LRAT.Formula.formulaHSat_def, List.all_eq_true, decide_eq_true_eq]
+    intro lratClause hlclause
+    simp only [LRAT.Formula.toList, LRAT.DefaultFormula.toList, LRAT.DefaultFormula.ofArray,
+      CNF.convertLRAT', Array.size_toArray, List.length_map, Array.toList_eq, Array.data_toArray,
+      List.map_nil, List.append_nil, List.mem_filterMap, List.mem_map, id_eq, exists_eq_right] at hlclause
+    rcases hlclause with ⟨reflectClause, ⟨hrclause1, hrclause2⟩⟩
+    simp only [CNF.eval, List.all_eq_true] at h3
+    simp [CNF.Clause.convertLRAT_sat_of_sat reflectClause hrclause2, h3 reflectClause hrclause1]
+  . contradiction
 
+/--
+Verify that a proof certificate is valid for a given `BoolExpr`.
 
+This is the verification function that we run in the reflection term.
+The advantage over running just `verifyCert` is that the Tseitin encoding happens
+in the reflection code as well instead of in the kernel reduction engine.
+-/
+def verifyBoolExpr (b : BoolExpr Nat) (cert : LratCert) : Bool :=
+  verifyCert (LratFormula.ofCnf b.toCNF) cert
+
+theorem unsat_of_verifyBoolExpr_eq_true (b : BoolExpr Nat) (c : LratCert)
+    (h : verifyBoolExpr b c = true) : BoolExpr.unsat b := by
+  apply BoolExpr.unsat_of_toCNF_unsat
+  apply verifyCert_correct
+  rw [verifyBoolExpr] at h
+  exact h
+
+/--
+Add an auxiliary declaration. Only used to create constants that appear in our reflection proof.
+-/
 def mkAuxDecl (name : Name) (value type : Expr) : MetaM Unit :=
   addAndCompile <| .defnDecl {
     name := name,
@@ -197,36 +190,47 @@ def mkAuxDecl (name : Name) (value type : Expr) : MetaM Unit :=
     safety := .safe
   }
 
-def lratSolver' (cfg : TacticConfig) (boolExpr : BoolExpr Nat) : MetaM Expr := do
+/--
+Prepare an `Expr` that proofs `boolExpr.unsat` using `ofReduceBool`.
+-/
+def lratSolver (cfg : TacticContext) (boolExpr : BoolExpr Nat) : MetaM Expr := do
   let cnf ←
     withTraceNode `sat (fun _ => return "Converting BoolExpr to CNF") do
       return boolExpr.toCNF
-  trace[sat] "Converted to CNF: {cnf}"
+
   let encoded ←
     withTraceNode `sat (fun _ => return "Converting frontend CNF to solver specific CNF") do
-      return lratSolver.encodeCNF cnf
+      return LratFormula.ofCnf cnf
+
   let cert ←
     withTraceNode `sat (fun _ => return "Obtaining external proof certificate") do
-      lratSolver.runExternal encoded
+      runExternal encoded
+
   withTraceNode `sat (fun _ => return "Compiling BoolExpr term") do
     mkAuxDecl cfg.boolExprDef (toExpr boolExpr) (toTypeExpr (BoolExpr Nat))
+
   let certType := toTypeExpr LratCert
+
   withTraceNode `sat (fun _ => return "Compiling proof certificate term") do
     mkAuxDecl cfg.certDef (toExpr cert) certType
 
   let boolExpr := mkConst cfg.boolExprDef
   let certExpr := mkConst cfg.certDef
-  let solverExpr := mkConst ``lratSolver
-  let cnfType := mkConst ``LratFormula
 
   withTraceNode `sat (fun _ => return "Compiling reflection proof term") do
-    let auxValue := mkApp5 (mkConst ``Solver.verifyExpr) cnfType certType solverExpr boolExpr certExpr
+    let auxValue := mkApp2 (mkConst ``verifyBoolExpr) boolExpr certExpr
     mkAuxDecl cfg.reflectionDef auxValue (mkConst ``Bool)
 
   let nativeProof := mkApp3 (mkConst ``Lean.ofReduceBool) (mkConst cfg.reflectionDef) (toExpr true) (← mkEqRefl (toExpr true))
-  return mkApp6 (mkConst ``Solver.unsat_of_verifyExpr_eq_true) cnfType certType solverExpr boolExpr certExpr nativeProof
+  return mkApp3 (mkConst ``unsat_of_verifyBoolExpr_eq_true) boolExpr certExpr nativeProof
 
-def _root_.Lean.MVarId.cnfDecide (g : MVarId) (cfg : TacticConfig) : MetaM Unit := M.run do
+/--
+Close a goal by turning:
+1. Turning it into a SAT problem.
+2. Running an external SAT solver on it and obtaining an LRAT proof from it.
+3. Verify the LRAT proof using proof by reflection.
+-/
+def _root_.Lean.MVarId.cnfDecide (g : MVarId) (cfg : TacticContext) : MetaM Unit := M.run do
   let g' ← falseOrByContra g
   g'.withContext do
     let (boolExpr, f) ←
@@ -235,14 +239,22 @@ def _root_.Lean.MVarId.cnfDecide (g : MVarId) (cfg : TacticConfig) : MetaM Unit 
     trace[sat] "Reflected boolean expression: {boolExpr}"
     let boolExprUnsat ←
       withTraceNode `sat (fun _ => return "Preparing LRAT reflection term") do
-        lratSolver' cfg boolExpr
+        lratSolver cfg boolExpr
     IO.println "before proof construction"
     let proveFalse ← f boolExprUnsat
     IO.println "after proof construction"
     g'.assign proveFalse
     IO.println "after assign"
 
+/--
+Close a goal by turning:
+1. Turning it into a SAT problem.
+2. Running an external SAT solver on it and obtaining an LRAT proof from it.
+3. Verify the LRAT proof using proof by reflection.
+-/
 syntax (name := cnfDecideSyntax) "cnf_decide" : tactic
+
+end CnfDecide
 
 open Elab.Tactic
 elab_rules : tactic
